A fix for helper functions in Selection
Problem:

 - In some respects, compartments create their own namespaces. Helper
   functions, in particular, have multiple copies, one per compartment.

 - In other respects, namespaces are unique. [AST.prog_defmap] in
   particular considers only names and hides all but the last copy of
   each helper function.

Solution:

 - Several possibilities. The simplest and most local seems to be
   selecting the helper functions from the list of program definitions
   instead of the map with shadowing. This fixes the compilation issues.

 - A cleaner if more invasive solution may involve starting from
   [AST.prog_defmap].

backend/Selection.v
@@ -484,10 +484,15 @@ Definition globdef_of_interest (gd: globdef) (cp: compartment) : bool :=
   | _ => false
   end.
 
-Definition record_globdefs (defmap: PTree.t globdef) (cp: compartment) : PTree.t globdef :=
-  PTree.fold
-    (fun m id gd => if globdef_of_interest gd cp then PTree.set id gd m else m)
-    defmap (PTree.empty globdef).
+(* Definition record_globdefs (defmap: PTree.t globdef) (cp: compartment) : PTree.t globdef := *)
+(*   PTree.fold *)
+(*     (fun m id gd => if globdef_of_interest gd cp then PTree.set id gd m else m) *)
+(*     defmap (PTree.empty globdef). *)
+
+Definition record_globdefs (defmap: Cminor.program) (cp: compartment) : PTree.t globdef :=
+  List.fold_left
+    (fun m '(id, gd) => if globdef_of_interest gd cp then PTree.set id gd m else m)
+    defmap.(prog_defs) (PTree.empty globdef).
 
 Definition lookup_helper_aux
      (cp: compartment) (name: String.string) (sg: signature) (res: option ident)
@@ -509,7 +514,8 @@ Definition lookup_helper (globs: PTree.t globdef)
 
 Local Open Scope string_scope.
 
-Definition get_helpers (defmap: PTree.t globdef) (cp: compartment): res helper_functions :=
+(* Definition get_helpers (defmap: PTree.t globdef) (cp: compartment): res helper_functions := *)
+Definition get_helpers (defmap: Cminor.program) (cp: compartment): res helper_functions :=
   let globs := record_globdefs defmap cp in
   do i64_dtos <- lookup_helper globs cp "__compcert_i64_dtos" sig_f_l ;
   do i64_dtou <- lookup_helper globs cp "__compcert_i64_dtou" sig_f_l ;
@@ -532,7 +538,8 @@ Definition get_helpers (defmap: PTree.t globdef) (cp: compartment): res helper_f
      i64_shl i64_shr i64_sar
      i64_umulh i64_smulh).
 
-Definition get_all_helpers (defmap: PTree.t globdef) (ls: list compartment): compartment -> res helper_functions :=
+(* Definition get_all_helpers (defmap: PTree.t globdef) (ls: list compartment): compartment -> res helper_functions := *)
+Definition get_all_helpers (defmap: Cminor.program) (ls: list compartment): compartment -> res helper_functions :=
   fun cp =>
     if @in_dec compartment Pos.eq_dec cp ls then
       do hf <- get_helpers defmap cp;
@@ -544,7 +551,12 @@ Definition get_all_helpers (defmap: PTree.t globdef) (ls: list compartment): com
 (** Conversion of programs. *)
 
 Definition sel_program (p: Cminor.program) : res program :=
+  (* FIXME: [prog_defmap] hides the multiple copies of the helper
+     functions, which share a name but live in different
+     compartments. A namespacing fix at that level may be worth
+     looking into. *)
   let dm := prog_defmap p in
-  let hf := get_all_helpers dm (AST.list_comp p) in
+  (* let hf := get_all_helpers dm (AST.list_comp p) in *)
+  let hf := get_all_helpers p (AST.list_comp p) in
   transform_partial_program (sel_fundef dm hf) p.
 
